theories/L6_PCPS/L4_to_L6_util.v
@@ -33,8 +33,8 @@ Section SUBSETS.
       S2 \subset S1.
 
   Definition cps_cvt_exps_subset_stmt :=
-    forall e e' k1 vars1 vs S1 S2,
-      cps_cvt_rel_exps func_tag kon_tag default_tag S1 e vars1 k1 vs cnstrs S2 e' ->
+    forall e e' k1 vars1 ks vs S1 S2,
+      cps_cvt_rel_exps func_tag kon_tag default_tag S1 e vars1 ks k1 vs cnstrs S2 e' ->
       S2 \subset S1.
 
   Definition cps_cvt_efnlst_subset_stmt :=
@@ -298,36 +298,39 @@ Section Post.
         preord_exp cenv P1 PG m (e1, rho1) (e2, rho2).
 
     Definition cps_cvt_exps_alpha_equiv k :=
-      forall es es1 es2 m k1 k2 vars1 vars2 xs1 xs2 ys1 ys2 rho1 rho2 S1 S2 S3 S4,
+      forall es es1 es2 m k1 k2 vars1 vars2 xs1 xs2 ks1 ks2 ys1 ys2 rho1 rho2 S1 S2 S3 S4,
         (m <= k)%nat ->
-        cps_cvt_rel_exps S1 es vars1 (Eapp k1 kon_tag (ys1 ++ xs1)) xs1 cnstrs S2 es1 ->
-        cps_cvt_rel_exps S3 es vars2 (Eapp k2 kon_tag (ys2 ++ xs2)) xs2 cnstrs S4 es2 ->
+        cps_cvt_rel_exps S1 es vars1 (Eapp k1 kon_tag (ys1 ++ xs1)) xs1 ks1 cnstrs S2 es1 ->
+        cps_cvt_rel_exps S3 es vars2 (Eapp k2 kon_tag (ys2 ++ xs2)) xs2 ks2 cnstrs S4 es2 ->
 
         NoDup vars1 ->
         NoDup xs1 ->
         NoDup xs2 ->
         NoDup ys1 ->
+        NoDup ks1 ->
         
 
         (* TODO some of these might be redundant *)
         
-        ~(k1 \in (FromList vars1 :|: FromList xs1 :|: FromList ys1)) ->
-        Disjoint _ (FromList vars1) (FromList xs1 :|: FromList ys1) -> 
+        ~(k1 \in (FromList vars1 :|: FromList xs1 :|: FromList ys1 :|: FromList ks1)) ->
+        Disjoint _ (FromList vars1) (FromList xs1 :|: FromList ys1 :|: FromList ks1) -> 
         
         List.length vars1 = List.length vars2 ->
         List.length xs1 = List.length xs2 ->
         List.length ys1 = List.length ys2 ->
         
-        Disjoint _ (k1 |: FromList vars1 :|: FromList xs1 :|: FromList ys1) S1 ->
-        Disjoint _ (k2 |: FromList vars2 :|: FromList xs2 :|: FromList ys2) S3 ->
-        Disjoint _ (FromList xs1) (FromList ys1) ->
-        Disjoint _ (FromList xs2) (k2 |: FromList vars2 :|: FromList ys2) ->
-        
+        Disjoint _ (k1 |: FromList vars1 :|: FromList xs1 :|: FromList ys1 :|: FromList ks1) S1 ->
+        Disjoint _ (k2 |: FromList vars2 :|: FromList xs2 :|: FromList ys2 :|: FromList ks2) S3 ->
+        Disjoint _ (FromList xs1 :|: FromList ks1) (FromList ys1) ->
+        Disjoint _ (FromList xs2 :|: FromList ks2) (k2 |: FromList vars2 :|: FromList ys2) ->
+        Disjoint _ (FromList xs1) (FromList ks1) ->
+        Disjoint _ (FromList xs2) (FromList ks2) ->
+
         preord_env_P_inj cenv PG (k1 |: FromList vars1 :|: FromList ys1 ) m
                          (id { k1 ~> k2 } <{ vars1 ~> vars2 }> <{ ys1 ~> ys2 }>) rho1 rho2 ->
         
         preord_exp cenv P1 PG m (es1, rho1) (es2, rho2). 
-
+    
     Definition cps_cvt_efnlst_alpha_equiv k :=
       forall efns fdefs1 fdefs2 m k1 k2 vars1 vars2 vars1' vars2' nlst1 nlst2 rho1 rho2
              S1 S2 S3 S4,
@@ -525,8 +528,8 @@ Section Post.
       end.
 
 
-    Lemma cps_cvt_rel_exps_len S1 es vars1 k1 xs1 S2 es1 :
-      cps_cvt_rel_exps S1 es vars1 k1 xs1 cnstrs S2 es1 ->
+    Lemma cps_cvt_rel_exps_len S1 es vars1 k1 xs1 ks1 S2 es1 :
+      cps_cvt_rel_exps S1 es vars1 k1 xs1 ks1 cnstrs S2 es1 ->
       List.length xs1 = N.to_nat (exps_length es).
     Proof.
       intros Hrel. induction Hrel; eauto.
@@ -536,7 +539,19 @@ Section Post.
         simpl. rewrite IHHrel.
         destruct p; lia.
     Qed.       
-    
+
+    Lemma cps_cvt_rel_exps_len_ks S1 es vars1 k1 xs1 ks1 S2 es1 :
+      cps_cvt_rel_exps S1 es vars1 k1 xs1 ks1 cnstrs S2 es1 ->
+      List.length ks1 = N.to_nat (exps_length es).
+    Proof.
+      intros Hrel. induction Hrel; eauto.
+      - simpl exps_length.
+        destruct (exps_length es) in *.
+        simpl; lia.
+        simpl. rewrite IHHrel.
+        destruct p; lia.
+    Qed.       
+
     Lemma cps_cvt_alpha_equiv :
       forall k, cps_cvt_alpha_equiv_statement k.
     Proof.
@@ -852,25 +867,39 @@ Section Post.
         + eapply Hprops. (* invariants *)
         + { eapply preord_exp_monotonic. eapply IH with (ys1 := []) (ys2 := []); simpl; try eassumption.
             - constructor.
-            - repeat normalize_sets. inv H4. intros Hc. inv Hc.
+            - repeat normalize_sets. inv H4. intros Hc. inv Hc. inv H2. 
               now eapply Hdis1; eauto.
-              eapply H6 in H2. inv H2. inv H4; eauto.
-            - repeat normalize_sets. eapply Disjoint_Included_r. eassumption. sets.
+              eapply H6 in H4. now inv_setminus; eauto.
+              eapply H7 in H2. now inv_setminus; eauto.
+            - repeat normalize_sets.
+              eapply Union_Disjoint_r. 
+              eapply Disjoint_Included_r. eassumption. now sets.
+              eapply Disjoint_Included_r. eassumption. now xsets.
             - erewrite !cps_cvt_rel_exps_len; eauto.
             - repeat normalize_sets. xsets.
-            - repeat normalize_sets. xsets.
-            - repeat normalize_sets. xsets.
+            - repeat normalize_sets.
+              eapply Union_Disjoint_l. now xsets. now sets.
+            - repeat normalize_sets.
+              eapply Union_Disjoint_l. now xsets. now sets.
             - repeat normalize_sets. xsets.
             - repeat normalize_sets. eapply Union_Disjoint_r; sets.
-              eapply Disjoint_Singleton_r. intros Hc. eapply H13 in Hc.
-              inv Hc; eauto. inv H0; eauto.
-              eapply Disjoint_Included_l. eassumption. sets.
+              eapply Disjoint_Singleton_r. intros Hc. inv Hc; eauto.              
+              eapply H15 in H0. now inv_setminus; eauto.
+              eapply H16 in H0. now inv_setminus; eauto.
+              eapply Disjoint_Included_l with (s3 := S3). 
+              eapply Union_Included. eapply Included_trans. sets. now sets.
+              eapply Included_trans. sets. now sets.
+              sets.
+            - repeat normalize_sets.
+              eapply Disjoint_Included_r. eassumption. xsets. 
+            - repeat normalize_sets.
+              eapply Disjoint_Included_r. eassumption. xsets. 
             - simpl.  
               assert (Hfeq : f_eq ((id {k3 ~> k4}) <{ vars1 ~> vars2 }>)
                                   ((id <{ vars1 ~> vars2 }>) {k3 ~> k4})). 
               { rewrite extend_extend_lst_commut; eauto. reflexivity. 
                 - inv H4. intros Hc. eapply Hdis1. sets.
-                - inv H11. intros Hc. eapply Hdis2. sets. }
+                - inv H13. intros Hc. eapply Hdis2. sets. }
               rewrite Hfeq.
               
               eapply preord_env_P_inj_set_alt; eauto.
@@ -898,7 +927,7 @@ Section Post.
                                (Fcons k4 kon_tag vx0 (Econstr x0 (dcon_to_tag default_tag dc cnstrs) vx0 (Eapp k2 kon_tag [x0])) Fnil)
                                (Fcons k4 kon_tag vx0 (Econstr x0 (dcon_to_tag default_tag dc cnstrs) vx0 (Eapp k2 kon_tag [x0])) Fnil)
                                rho2 rho2); [ | | now eauto | ].
-                rewrite H7. rewrite H14. reflexivity. eassumption. 
+                rewrite H8. rewrite H17. reflexivity. eassumption. 
                 
                 eexists. split. now eauto. 
 
@@ -946,18 +975,18 @@ Section Post.
                       * intros Hc. eapply image_extend_lst_Included in Hc.
                         inv Hc.
                         
-                        eapply image_extend_Included' in H17. 
-                        rewrite image_id in H17.
+                        eapply image_extend_Included' in H21. 
+                        rewrite image_id in H21.
 
-                        rewrite Setminus_Union_distr, Setminus_Same_set_Empty_set in H17.
+                        rewrite Setminus_Union_distr, Setminus_Same_set_Empty_set in H21.
                         repeat normalize_sets.
-                        rewrite Setminus_Union, (Union_commut (FromList vars1)), <- Setminus_Union, Setminus_Same_set_Empty_set in H17.
+                        rewrite Setminus_Union, (Union_commut (FromList vars1)), <- Setminus_Union, Setminus_Same_set_Empty_set in H21.
                         repeat normalize_sets. 
-                        inv H17. inv H11. eapply Hdis2. now sets.
-                        inv H11. eapply Hdis2. now sets.
+                        inv H21. inv H13. eapply Hdis2. now sets.
+                        inv H13. eapply Hdis2. now sets.
                         eassumption.
                         
-                      * intros Hc. inv Hc. inv H17.
+                      * intros Hc. inv Hc. inv H21.
                         inv H4. eapply Hdis1. now sets.
                         inv H4. eapply Hdis1. now sets.
                         
@@ -974,7 +1003,7 @@ Section Post.
                         rewrite image_id.
                         rewrite Setminus_Same_set_Empty_set. now sets.
 
-                        eapply Disjoint_Singleton_r. intros Hc. eapply H12 in Hc. inv_setminus. 
+                        eapply Disjoint_Singleton_r. intros Hc. eapply H14 in Hc. inv_setminus. 
                         now eapply Hdis2; eauto.
                         
                         eapply Disjoint_sym. eapply Disjoint_Included; [ | | eapply Hdis2 ].
@@ -989,15 +1018,17 @@ Section Post.
 
                       * intros Hc.
                         eapply image_extend_lst_Included in Hc. inv Hc.
-                        rewrite Setminus_Union_distr, Setminus_Same_set_Empty_set in H17.
+                        rewrite Setminus_Union_distr, Setminus_Same_set_Empty_set in H21.
                         repeat normalize_sets.
-                        eapply image_extend_Included' in H17. rewrite image_id in H17.
-                        inv H17. inv H19. inv H17. now eauto.
-                        inv H19. eapply Hdis2. now sets.
+                        eapply image_extend_Included' in H21. rewrite image_id in H21.
+                        inv H21. inv H23. inv H21. now eauto.
+                        inv H22. eapply Hdis2. now sets.
                         eapply Hdis2. now sets.
+                        eapply Hdis2. now sets.
+
                         eassumption.
 
-                      * intros Hc. inv Hc. inv H17. 
+                      * intros Hc. inv Hc. inv H21. 
                         eapply Hdis1; now sets.
                         eapply Hdis1; now sets.
 
@@ -1014,7 +1045,7 @@ Section Post.
 
                 rewrite image_id in H0. inv H0. now inv H1.
                 
-                inv H11. eapply Hdis2. constructor; now eauto. eassumption.
+                inv H13. eapply Hdis2. constructor; now eauto. eassumption.
                 
             - lia. }
           
@@ -1335,16 +1366,18 @@ Section Post.
         (* TODO add Prim_e to relation ? *)
         
       - (* enil *)
-        intros es1 es2 m k1 k2 vars1 vars2 xs1 xs2 ys1 ys2 rho1 rho2 S1 S2 S3 S4
-               Hm He1 He2 Hdup Hdup' Hdup'' Hdup''' Hnot Hdis Hlen Hlen' Hlen'' Hdis1 Hdis2 Hdis3 Hdis4 Henv.
+        intros es1 es2 m k1 k2 vars1 vars2 xs1 xs2 ks1 ks2 ys1 ys2 rho1 rho2 S1 S2 S3 S4
+               Hm He1 He2 Hdup1 Hdup2 Hdup3 Hdup4 Hnd5 Hnot Hdis Hlen Hlen' Hlen''
+               Hdis1 Hdis2 Hdis3 Hdis4 Hdis5 Hdis6 Henv.
         inv He1; inv He2.
         eapply preord_exp_app_compat; simpl.
         + eapply Hprops. (* invariants *)
         + eapply Hprops. (* invariants *)
-        + repeat normalize_sets.
+        + rewrite FromList_nil in Hdis1 at 1. 
           assert (Heq: k2 = (((id {k1 ~> k2}) <{ vars1 ~> vars2 }>) <{ ys1 ~> ys2 }>) k1).
-          { rewrite extend_lst_gso. rewrite extend_lst_gso. rewrite extend_gss. reflexivity. now eauto.
-            now sets. } 
+          { rewrite extend_lst_gso. rewrite extend_lst_gso. rewrite extend_gss. reflexivity.
+            intros Hc. eapply Hnot; eauto.
+            intros Hc. eapply Hnot; eauto. } 
           rewrite Heq. eapply Henv. now left.
         + simpl. rewrite !app_nil_r.
           erewrite <- map_extend_lst_same with (xs := ys1) (xs' := ys2).
@@ -1352,19 +1385,21 @@ Section Post.
           eassumption. eassumption. 
           
       - (* econs *) 
-        intros e IHe es IHes e1 e2 m k1 k2 vars1 vars2 xs1 xs2 ys1 ys2 rho1 rho2 S1 S2 S3 S4
-               Hm He1 He2 Hdup Hdup' Hdup'' Hdup'''  Hnot Hdis Hlen Hlen' Hlen'' Hdis1 Hdis2 Hdis3 Hdis4 Henv.
+        intros e IHe es IHes e1 e2 m k1 k2 vars1 vars2 xs1 xs2 ys1 ys2 ks1 ks2 rho1 rho2 S1 S2 S3 S4
+               Hm He1 He2 Hdup1 Hdup2 Hdup3 Hdup4 Hnd5  Hnot Hdis Hlen Hlen' Hlen''
+               Hdis1 Hdis2 Hdis3 Hdis4 Hdis5 Hdis6 Henv.
         inv He1; inv He2. 
         eapply preord_exp_fun_compat.
         + eapply Hprops. (* invariants *)
         + eapply Hprops. (* invariants *)
         + { simpl. eapply preord_exp_monotonic.
             eapply IHe; try eassumption.
-            - intros Hc. eapply Hdis1. sets.
-            - xsets. 
-            - xsets.
+            - repeat normalize_sets. intros Hc.
+              eapply Hdis; eauto. 
+            - repeat normalize_sets. xsets.
+            - repeat normalize_sets. xsets.
             - simpl. rewrite extend_extend_lst_commut; eauto.
-              + eapply preord_env_P_inj_set_alt.
+              + eapply preord_env_P_inj_set_alt. 
                 * rewrite Setminus_Union_distr.
                   rewrite Setminus_Same_set_Empty_set. normalize_sets.
                   eapply preord_env_P_inj_f_eq_subdomain.
@@ -1390,15 +1425,18 @@ Section Post.
                     eapply preord_exp_monotonic.
                     eapply preord_exp_post_monotonic. eapply HinclG. 
                     edestruct (H j) as (_ & Hexps & _ & _ ). lia.
-                    rewrite <- MCList.app_tip_assoc in H11, H14. inv Hdup'.
+                    rewrite <- MCList.app_tip_assoc in H11, H13. inv Hdup2.
                     repeat normalize_sets.
                     eapply Hexps; try eassumption.
                     - reflexivity.
-                    - inv Hdup''. eassumption.
+                    - inv Hdup3. eassumption.
                     - eapply NoDup_app. eassumption. constructor. intros Hc. now inv Hc. now constructor.  
                       repeat normalize_sets. sets.
-                    - repeat normalize_sets. intros Hc; inv Hc; eauto. inv H1; eauto. inv H1; eauto.
-                    - repeat normalize_sets. sets.
+                    - inv Hnd5; eauto.
+                    - repeat normalize_sets. intros Hc; inv Hc; eauto.
+                      eapply Hnot. inv H1; eauto. inv H2; eauto. inv H2; eauto.
+                      
+                    - repeat normalize_sets. xsets.
                     - congruence.
                     - rewrite !app_length. simpl. congruence.
                     - repeat normalize_sets. eapply Disjoint_Included_r.
@@ -1407,13 +1445,21 @@ Section Post.
                     - repeat normalize_sets. eapply Disjoint_Included_r.
                       eapply cps_cvt_exp_subset. eassumption. repeat normalize_sets. xsets.
 
-                    - repeat normalize_sets. sets.
+                    - repeat normalize_sets.
+                      eapply Union_Disjoint_l; sets.
+                      eapply Union_Disjoint_r; sets.
+                      eapply Disjoint_sym. eapply Disjoint_Included; [ | | eapply Hdis5 ]; sets. 
                     - repeat normalize_sets. 
                       rewrite !Union_assoc. 
                       eapply Union_Disjoint_r.
                       eapply Disjoint_Included; [ | | eapply Hdis4 ]; now sets.
-                      inv Hdup''. eapply Disjoint_Singleton_r. eassumption.
-                      
+                      inv Hdup3. eapply Disjoint_Singleton_r.
+                      intros Hc; inv Hc; eauto.
+                      now eapply Hdis6 ; eauto.
+                    - repeat normalize_sets.
+                      eapply Disjoint_Included; [ | | eapply Hdis5 ]; sets.
+                    - repeat normalize_sets.
+                      eapply Disjoint_Included; [ | | eapply Hdis6 ]; sets.
                     - simpl. rewrite !extend_lst_app; eauto. simpl.
                       rewrite extend_extend_lst_commut.
                       
@@ -1428,31 +1474,31 @@ Section Post.
                         2: { eassumption. } lia.
                         repeat normalize_sets. now xsets.
                         
-                        * repeat normalize_sets. intros Hc. inv Hc; eauto.
-                          inv H1; eauto. inv H9. inv H1. now eapply Hdis1; eauto.
-                          now eapply Hdis1; eauto.
-                          inv H9; eauto.
-                          now eapply Hdis1; eauto.
+                        * repeat normalize_sets.
+                          intros Hc. inv Hnd5. inv Hc; eauto.
+                          inv H1; eauto. inv H12; eauto. inv H1; now eauto.
+                          now eapply Hdis; eauto.
+                          inv H12; eauto. eapply Hdis3. eauto. 
                           
                         * intros Hc. eapply image_extend_lst_Included in Hc; eauto.
-                          inv Hc; eauto.
+                          inv Hc; eauto. 
 
                           eapply image_extend_lst_Included in H1; eauto.
 
                           inv H1.
-                          eapply image_extend_Included' in H5. 
-                          rewrite image_id in H5.
-                          repeat normalize_sets. inv H5. 
+                          eapply image_extend_Included' in H2. 
+                          rewrite image_id in H2.
+                          repeat normalize_sets. inv H2. 
                           
                           
-                          assert (Heq : (k1 |: FromList vars1 :|: (FromList ys1 :|: [set x1]) \\ [set x1] \\
-                                            FromList ys1 \\ FromList vars1 \\ [set k1]) <--> Empty_set _) by xsets.
+                          assert (Heq : (k1 |: FromList vars1 :|: (FromList ks1 :|: [set x1]) \\ [set x1] \\
+                                            FromList ks1 \\ FromList vars1 \\ [set k1]) <--> Empty_set _) by xsets.
                           
                           eapply Heq in H1. now inv H1.
-                          
-                          inv H1. now eapply Hdis2; eauto.
-                          now eapply Hdis2; eauto.
-                          now eapply Hdis2; eauto. 
+                          (* inv H1.  *)
+                          inv H1. eapply Hdis4. constructor. right. now left. now left.
+                          eapply Hdis4; eauto. constructor. right. now left. left. now right.
+                          eapply Hdis4; eauto.
 
                         * intros Hc. eapply image_extend_lst_Included in Hc; eauto.
                           inv Hc; eauto.
@@ -1460,18 +1506,18 @@ Section Post.
                           eapply image_extend_lst_Included in H1; eauto.
 
                           inv H1.
-                          eapply image_extend_Included' in H5. 
-                          rewrite image_id in H5.
-                          repeat normalize_sets. inv H5. 
+                          eapply image_extend_Included' in H2. 
+                          rewrite image_id in H2.
+                          repeat normalize_sets. inv H2. 
 
                           
-                          assert (Heq : (k1 |: FromList vars1 :|: (FromList ys1 :|: [set x1]) \\ [set x1] \\
-                                            FromList ys1 \\ FromList vars1 \\ [set k1]) <--> Empty_set _) by xsets.
+                          assert (Heq : (k1 |: FromList vars1 :|: (FromList ks1 :|: [set x1]) \\ [set x1] \\
+                                            FromList ks1 \\ FromList vars1 \\ [set k1]) <--> Empty_set _) by xsets.
 
                           eapply  Heq in H1. now inv H1.
-                          inv H1; eapply Hdis4; now eauto.
-                          eapply Hdis4; now eauto.
-                          eapply Hdis4; now eauto.
+                          inv H1; eapply Hdis4. constructor. left. now left. now eauto.
+                          eapply Hdis4. constructor. left. now left. now eauto.
+                          eapply Hdis4. constructor. left. now left. now eauto.
                           
                       + intros Hc; eapply Hdis3; eauto.
                         
@@ -1487,12 +1533,13 @@ Section Post.
                   rewrite image_id in Hc. inv Hc.
 
                   inv H0. inv H1; now eauto.
-
-                  now eapply Hdis2; eauto.
                   
-              + intros Hc. eapply Hdis1; eauto.
+                  eapply Hdis4. constructor. right. now left. now eauto.
+                  
+              + repeat normalize_sets. intros Hc.
+                eapply Hdis; eauto.
                 
-              + intros Hc. eapply Hdis2; eauto.
+              + repeat normalize_sets. intros Hc. eapply Hdis4. constructor. right. now left. eauto.
                 
             - lia. } 
           
